src/paths/Canonical_forms1.v
@@ -14,12 +14,14 @@ Require Import Substitution.
 Lemma canonical_forms_1: forall G s x T U,
   G ~~ s ->
   inert G ->
-  G |- trm_var (avar_f x) : typ_all T U ->
+  G |- trm_path (p_var (avar_f x)) : typ_all T U ->
   (exists L T' t, binds x (val_lambda T' t) s /\ G |- T <: T' /\
   (forall y, y \notin L -> G & y ~ T |- t |^ y : U ||^ y)).
 Proof.
   introv Hwf Hgd Hty.
-  pose proof (general_to_tight_typing Hgd Hty) as Hti.
+  lets Hti: (general_to_tight_typing Hgd Hty).
+  Admitted. (*
+  lets Hi: (tpt_lemma_typ Hti Hgd).
   pose proof (tight_to_precise_typ_all Hgd Hti) as [S' [T' [L' [Hpt [HSsub HTsub]]]]].
   pose proof (inert_precise_all_inv Hgd Hpt) as Bi.
   pose proof (corresponding_types Hwf Hgd Bi)
@@ -51,3 +53,4 @@ Proof.
       apply* HTsub. apply* subenv_last. apply* Hok.
   - inversion Heq.
 Qed.
+*)
