src/paths/General_to_tight.v
@@ -11,13 +11,13 @@ Require Import Tight_possible_types.
 (* Lemma 2 *)
 Lemma tight_subtyping_sel: forall G p A S U,
     inert G ->
-    norm_t G p ->
+    G |-# p \||/ ->
     G |-# trm_path p : typ_rcd { A >: S <: U } ->
     G |-# typ_path p A <: U /\
     G |-# S <: typ_path p A.
 Proof.
   introv Hi Hn Hty.
-  lets Hp: (tight_possible_types_lemma Hi Hty Hn).
+  lets Hp: (tpt_lemma_typ Hty Hi Hn).
   pose proof (tpt_to_precise_typ_dec Hi Hn Hp) as [T [Ht [Hs1 Hs2]]].
   split.
   - apply subtyp_sel1_t in Ht. apply subtyp_trans_t with (T:=T); auto. assumption.
